Add some additional core models.

hax-lib/core-models/src/core/clone.rs
@@ -1,0 +1,10 @@
+trait Clone {
+    fn clone(self) -> Self;
+}
+
+// In our model, everything is clonable
+impl<T> Clone for T {
+    fn clone(self) -> Self {
+        self
+    }
+}
