hax-lib/core-models/src/core/convert.rs
@@ -1,0 +1,59 @@
+use super::result::Result;
+
+trait TryInto<T> {
+    type Error;
+    fn try_into(self) -> Result<T, Self::Error>;
+}
+
+trait Into<T> {
+    fn into(self) -> T;
+}
+
+trait From<T> {
+    fn from(x: T) -> Self;
+}
+
+trait TryFrom<T>: Sized {
+    type Error;
+    fn try_from(x: T) -> Result<Self, Self::Error>;
+}
+
+// Need manual definitions for integer types. Need definition of Infallible
+
+impl<T, U: From<T>> Into<U> for T {
+    fn into(self) -> U {
+        U::from(self)
+    }
+}
+
+pub struct Infallible;
+
+impl<T, U: From<T>> TryFrom<T> for U {
+    type Error = Infallible;
+    fn try_from(x: T) -> Result<Self, Self::Error> {
+        Result::Ok(U::from(x))
+    }
+}
+
+impl<T, U: TryFrom<T>> TryInto<U> for T {
+    type Error = U::Error;
+    fn try_into(self) -> Result<U, Self::Error> {
+        U::try_from(self)
+    }
+}
+
+impl<T> From<T> for T {
+    fn from(x: T) -> Self {
+        x
+    }
+}
+
+trait AsRef<T> {
+    fn as_ref(self) -> T;
+}
+
+impl<T> AsRef<T> for T {
+    fn as_ref(self) -> T {
+        self
+    }
+}
