hax-lib/core-models/src/core/hint.rs
@@ -1,0 +1,7 @@
+pub const fn black_box<T>(dummy: T) -> T {
+    dummy
+}
+
+pub const fn must_use<T>(value: T) -> T {
+    value
+}
