hax-lib/core-models/src/core/mem.rs
@@ -1,5 +1,12 @@
-#[hax_lib::ensures(|res| res == old(dest) && dest == src)]
+#![allow(unused_variables)]
+
 #[hax_lib::opaque]
 pub fn replace<T>(dest: &mut T, src: T) -> T {
     panic!()
+}
+
+mod manually_drop {
+    pub struct ManuallyDrop<T: ?Sized> {
+        value: T,
+    }
 }
