hax-lib/proof-libs/fstar/core/Core_models.Clone.fst
@@ -1,15 +1,18 @@
 module Core_models.Clone
+#set-options "--fuel 0 --ifuel 1 --z3rlimit 15"
+open Core
+open FStar.Mul
 
-class t_Clone self = {
-  f_clone_pre: self -> Type0;
-  f_clone_post: self -> self -> Type0;
-  f_clone: x:self -> r:self {x == r}
+class t_Clone (v_Self: Type0) = {
+  f_clone_pre:v_Self -> Type0;
+  f_clone_post:v_Self -> v_Self -> Type0;
+  f_clone:x0: v_Self -> Prims.Pure v_Self (f_clone_pre x0) (fun result -> f_clone_post x0 result)
 }
 
-(** Everything is clonable *)
-instance clone_all (t: Type): t_Clone t = {
-  f_clone_pre = (fun _ -> True);
-  f_clone_post = (fun _ _ -> True);
-  f_clone = (fun x -> x);
-}
-
+[@@ FStar.Tactics.Typeclasses.tcinstance]
+let impl (#v_T: Type0) : t_Clone v_T =
+  {
+    f_clone_pre = (fun (self: v_T) -> true);
+    f_clone_post = (fun (self: v_T) (out: v_T) -> true);
+    f_clone = fun (self: v_T) -> self
+  }
