hax-lib/proof-libs/fstar/core/Core_models.Error.fsti
@@ -1,9 +1,23 @@
 module Core_models.Error
-
+#set-options "--fuel 0 --ifuel 1 --z3rlimit 15"
+open Core
 open FStar.Mul
 
-class t_Error (v_Self: Type0) = {
-  [@@@ FStar.Tactics.Typeclasses.no_method]_super_1049815079118268934:Core_models.Fmt.t_Debug v_Self;
-  [@@@ FStar.Tactics.Typeclasses.no_method]_super_15857421111036552015:Core_models.Fmt.t_Display v_Self;
+let _ =
+  (* This module has implicit dependencies, here we make them explicit. *)
+  (* The implicit dependencies arise from typeclasses instances. *)
+  let open Core_models.Fmt in
+  ()
 
+class t_Error (v_Self: Type0) = {
+  [@@@ FStar.Tactics.Typeclasses.no_method]_super_6821900375476161560:Core_models.Fmt.t_Display
+  v_Self;
+  [@@@ FStar.Tactics.Typeclasses.no_method]_super_14599973916339107634:Core_models.Fmt.t_Debug
+  v_Self
 }
+
+[@@ FStar.Tactics.Typeclasses.tcinstance]
+let _ = fun (v_Self:Type0) {|i: t_Error v_Self|} -> i._super_6821900375476161560
+
+[@@ FStar.Tactics.Typeclasses.tcinstance]
+let _ = fun (v_Self:Type0) {|i: t_Error v_Self|} -> i._super_14599973916339107634
