hax-lib/proof-libs/fstar/core/Core_models.Num.Error.fsti
@@ -1,6 +1,75 @@
 module Core_models.Num.Error
-open Rust_primitives
+#set-options "--fuel 0 --ifuel 1 --z3rlimit 15"
+open Core
+open FStar.Mul
 
-type t_ParseIntError = unit
-type t_TryFromIntError = unit
+let _ =
+  (* This module has implicit dependencies, here we make them explicit. *)
+  (* The implicit dependencies arise from typeclasses instances. *)
+  let open Core_models.Fmt in
+  ()
 
+/// The error type returned when a checked integral type conversion fails.
+type t_TryFromIntError = | TryFromIntError : Prims.unit -> t_TryFromIntError
+
+val f_fmt__impl__panic_cold_explicit: Prims.unit
+  -> Prims.Pure Rust_primitives.Hax.t_Never Prims.l_True (fun _ -> Prims.l_True)
+
+[@@ FStar.Tactics.Typeclasses.tcinstance]
+val impl:Core_models.Fmt.t_Display t_TryFromIntError
+
+[@@ FStar.Tactics.Typeclasses.tcinstance]
+val impl_1:Core_models.Error.t_Error t_TryFromIntError
+
+val f_from__impl_2__panic_cold_explicit: Prims.unit
+  -> Prims.Pure Rust_primitives.Hax.t_Never Prims.l_True (fun _ -> Prims.l_True)
+
+[@@ FStar.Tactics.Typeclasses.tcinstance]
+val impl_2:Core.Convert.t_From t_TryFromIntError Core_models.Convert.t_Infallible
+
+/// Enum to store the various types of errors that can cause parsing an integer to fail.
+/// # Example
+/// ```
+/// # fn main() {
+/// if let Err(e) = i32::from_str_radix("a12", 10) {
+///     println!("Failed conversion to i32: {:?}", e.kind());
+/// }
+/// # }
+/// ```
+type t_IntErrorKind =
+  | IntErrorKind_Empty : t_IntErrorKind
+  | IntErrorKind_InvalidDigit : t_IntErrorKind
+  | IntErrorKind_PosOverflow : t_IntErrorKind
+  | IntErrorKind_NegOverflow : t_IntErrorKind
+  | IntErrorKind_Zero : t_IntErrorKind
+
+/// An error which can be returned when parsing an integer.
+/// This error is used as the error type for the `from_str_radix()` functions
+/// on the primitive integer types, such as [`i8::from_str_radix`].
+/// # Potential causes
+/// Among other causes, `ParseIntError` can be thrown because of leading or trailing whitespace
+/// in the string e.g., when it is obtained from the standard input.
+/// Using the [`str::trim()`] method ensures that no whitespace remains before parsing.
+/// # Example
+/// ```
+/// if let Err(e) = i32::from_str_radix("a12", 10) {
+///     println!("Failed conversion to i32: {e}");
+/// }
+/// ```
+type t_ParseIntError = { f_kind:t_IntErrorKind }
+
+val t_IntErrorKind_cast_to_repr (x: t_IntErrorKind)
+    : Prims.Pure isize Prims.l_True (fun _ -> Prims.l_True)
+
+/// Outputs the detailed cause of parsing an integer failing.
+val impl_ParseIntError__kind (self: t_ParseIntError)
+    : Prims.Pure t_IntErrorKind Prims.l_True (fun _ -> Prims.l_True)
+
+val f_fmt__impl_4__panic_cold_explicit: Prims.unit
+  -> Prims.Pure Rust_primitives.Hax.t_Never Prims.l_True (fun _ -> Prims.l_True)
+
+[@@ FStar.Tactics.Typeclasses.tcinstance]
+val impl_4:Core_models.Fmt.t_Display t_ParseIntError
+
+[@@ FStar.Tactics.Typeclasses.tcinstance]
+val impl_5:Core_models.Error.t_Error t_ParseIntError
