hax-lib/proof-libs/fstar/core/Core_models.Ops.Control_flow.fst
@@ -1,6 +1,8 @@
 module Core_models.Ops.Control_flow
+#set-options "--fuel 0 --ifuel 1 --z3rlimit 15"
+open Core
+open FStar.Mul
 
-type t_ControlFlow (b c: Type) = 
-  | ControlFlow_Continue of c
-  | ControlFlow_Break of b
-
+type t_ControlFlow (v_C: Type0) (v_B: Type0) =
+  | ControlFlow_Continue : v_C -> t_ControlFlow v_C v_B
+  | ControlFlow_Break : v_B -> t_ControlFlow v_C v_B
