hax-lib/proof-libs/fstar/core/Core_models.Option.fst
@@ -1,6 +1,14 @@
 module Core_models.Option
 #set-options "--fuel 0 --ifuel 1 --z3rlimit 15"
+open Core
 open FStar.Mul
+
+let _ =
+  (* This module has implicit dependencies, here we make them explicit. *)
+  (* The implicit dependencies arise from typeclasses instances. *)
+  let open Core_models.Default in
+  let open Core_models.Ops.Function in
+  ()
 
 type t_Option (v_T: Type0) =
   | Option_Some : v_T -> t_Option v_T
@@ -11,7 +19,6 @@ open Rust_primitives.Integers
 let impl__is_some_and
       (#v_T #v_F: Type0)
       (#[FStar.Tactics.Typeclasses.tcresolve ()] i0: Core_models.Ops.Function.t_FnOnce v_F v_T)
-      (#_: unit{i0.Core_models.Ops.Function.f_Output == bool})
       (self: t_Option v_T)
       (f: v_F)
     : bool =
@@ -23,7 +30,6 @@ let impl__is_some_and
 let impl__is_none_or
       (#v_T #v_F: Type0)
       (#[FStar.Tactics.Typeclasses.tcresolve ()] i0: Core_models.Ops.Function.t_FnOnce v_F v_T)
-      (#_: unit{i0.Core_models.Ops.Function.f_Output == bool})
       (self: t_Option v_T)
       (f: v_F)
     : bool =
@@ -47,7 +53,6 @@ let impl__unwrap_or_else
       (#[FStar.Tactics.Typeclasses.tcresolve ()]
           i1:
           Core_models.Ops.Function.t_FnOnce v_F Prims.unit)
-      (#_: unit{i1.Core_models.Ops.Function.f_Output == v_T})
       (self: t_Option v_T)
       (f: v_F)
     : v_T =
@@ -72,7 +77,6 @@ let impl__unwrap_or_default
 let impl__map
       (#v_T #v_U #v_F: Type0)
       (#[FStar.Tactics.Typeclasses.tcresolve ()] i3: Core_models.Ops.Function.t_FnOnce v_F v_T)
-      (#_: unit{i3.Core_models.Ops.Function.f_Output == v_U})
       (self: t_Option v_T)
       (f: v_F)
     : t_Option v_U =
@@ -87,7 +91,6 @@ let impl__map
 let impl__map_or
       (#v_T #v_U #v_F: Type0)
       (#[FStar.Tactics.Typeclasses.tcresolve ()] i3: Core_models.Ops.Function.t_FnOnce v_F v_T)
-      (#_: unit{i3.Core_models.Ops.Function.f_Output == v_U})
       (self: t_Option v_T)
       (v_default: v_U)
       (f: v_F)
@@ -100,11 +103,9 @@ let impl__map_or
 let impl__map_or_else
       (#v_T #v_U #v_D #v_F: Type0)
       (#[FStar.Tactics.Typeclasses.tcresolve ()] i4: Core_models.Ops.Function.t_FnOnce v_F v_T)
-      (#_: unit{i4.Core_models.Ops.Function.f_Output == v_U})
       (#[FStar.Tactics.Typeclasses.tcresolve ()]
           i5:
           Core_models.Ops.Function.t_FnOnce v_D Prims.unit)
-      (#_: unit{i5.Core_models.Ops.Function.f_Output == v_U})
       (self: t_Option v_T)
       (v_default: v_D)
       (f: v_F)
@@ -122,7 +123,6 @@ let impl__map_or_else
 let impl__map_or_default
       (#v_T #v_U #v_F: Type0)
       (#[FStar.Tactics.Typeclasses.tcresolve ()] i3: Core_models.Ops.Function.t_FnOnce v_F v_T)
-      (#_: unit{i3.Core_models.Ops.Function.f_Output == v_U})
       (#[FStar.Tactics.Typeclasses.tcresolve ()] i6: Core_models.Default.t_Default v_U)
       (self: t_Option v_T)
       (f: v_F)
@@ -143,7 +143,6 @@ let impl__ok_or_else
       (#[FStar.Tactics.Typeclasses.tcresolve ()]
           i7:
           Core_models.Ops.Function.t_FnOnce v_F Prims.unit)
-      (#_: unit{i7.Core_models.Ops.Function.f_Output == v_E})
       (self: t_Option v_T)
       (err: v_F)
     : Core_models.Result.t_Result v_T v_E =
@@ -162,7 +161,6 @@ let impl__ok_or_else
 let impl__and_then
       (#v_T #v_U #v_F: Type0)
       (#[FStar.Tactics.Typeclasses.tcresolve ()] i3: Core_models.Ops.Function.t_FnOnce v_F v_T)
-      (#_: unit{i3.Core_models.Ops.Function.f_Output == t_Option v_U})
       (self: t_Option v_T)
       (f: v_F)
     : t_Option v_U =
