hax-lib/proof-libs/fstar/core/Core_models.Result.fst
@@ -1,6 +1,13 @@
 module Core_models.Result
 #set-options "--fuel 0 --ifuel 1 --z3rlimit 15"
+open Core
 open FStar.Mul
+
+let _ =
+  (* This module has implicit dependencies, here we make them explicit. *)
+  (* The implicit dependencies arise from typeclasses instances. *)
+  let open Core_models.Ops.Function in
+  ()
 
 type t_Result (v_T: Type0) (v_E: Type0) =
   | Result_Ok : v_T -> t_Result v_T v_E
@@ -9,7 +16,6 @@ type t_Result (v_T: Type0) (v_E: Type0) =
 let impl__map
       (#v_T #v_E #v_U #v_F: Type0)
       (#[FStar.Tactics.Typeclasses.tcresolve ()] i0: Core_models.Ops.Function.t_FnOnce v_F v_T)
-      (#_: unit{i0.Core_models.Ops.Function.f_Output == v_U})
       (self: t_Result v_T v_E)
       (op: v_F)
     : t_Result v_U v_E =
@@ -23,7 +29,6 @@ let impl__map
 let impl__map_or
       (#v_T #v_E #v_U #v_F: Type0)
       (#[FStar.Tactics.Typeclasses.tcresolve ()] i0: Core_models.Ops.Function.t_FnOnce v_F v_T)
-      (#_: unit{i0.Core_models.Ops.Function.f_Output == v_U})
       (self: t_Result v_T v_E)
       (v_default: v_U)
       (f: v_F)
@@ -31,14 +36,12 @@ let impl__map_or
   match self <: t_Result v_T v_E with
   | Result_Ok t ->
     Core_models.Ops.Function.f_call_once #v_F #v_T #FStar.Tactics.Typeclasses.solve f t
-  | Result_Err e -> v_default
+  | Result_Err e_e -> v_default
 
 let impl__map_or_else
       (#v_T #v_E #v_U #v_D #v_F: Type0)
       (#[FStar.Tactics.Typeclasses.tcresolve ()] i1: Core_models.Ops.Function.t_FnOnce v_F v_T)
-      (#_: unit{i1.Core_models.Ops.Function.f_Output == v_U})
       (#[FStar.Tactics.Typeclasses.tcresolve ()] i2: Core_models.Ops.Function.t_FnOnce v_D v_E)
-      (#_: unit{i2.Core_models.Ops.Function.f_Output == v_U})
       (self: t_Result v_T v_E)
       (v_default: v_D)
       (f: v_F)
@@ -52,7 +55,6 @@ let impl__map_or_else
 let impl__map_err
       (#v_T #v_E #v_O #v_F: Type0)
       (#[FStar.Tactics.Typeclasses.tcresolve ()] i3: Core_models.Ops.Function.t_FnOnce v_O v_E)
-      (#_: unit{i3.Core_models.Ops.Function.f_Output == v_F})
       (self: t_Result v_T v_E)
       (op: v_O)
     : t_Result v_T v_F =
@@ -72,7 +74,6 @@ let impl__is_ok (#v_T #v_E: Type0) (self: t_Result v_T v_E) : bool =
 let impl__and_then
       (#v_T #v_E #v_U #v_F: Type0)
       (#[FStar.Tactics.Typeclasses.tcresolve ()] i0: Core_models.Ops.Function.t_FnOnce v_F v_T)
-      (#_: unit{i0.Core_models.Ops.Function.f_Output == t_Result v_U v_E})
       (self: t_Result v_T v_E)
       (op: v_F)
     : t_Result v_U v_E =
